src/FcEtt/fc_get.v
@@ -250,12 +250,12 @@ Proof.
       move: (binds_unique _ _ _ _ _ H2 P uniq_an_toplevel) => h0. inversion h0.
       move: (binds_unique _ _ _ _ _ H2 P uniq_an_toplevel) => h0. inversion h0. auto.
       eapply NB in H2. done.
-    - inversion HT. subst. Opaque an_toplevel.
+(*    - inversion HT. subst. Opaque an_toplevel.
       simpl.
       destruct (binds_lookup _ T an_toplevel) as [ [ [A0 | phi] P] | NB].
       move: (binds_unique _ _ _ _ _ H2 P uniq_an_toplevel) => h0. inversion h0. auto.
       move: (binds_unique _ _ _ _ _ H2 P uniq_an_toplevel) => h0. inversion h0.
-      eapply NB in H2. done.
+      eapply NB in H2. done. *)
     - inversion HT. subst. simpl.
       remember (get_deq_n n G g) as GD. destruct GD as [A' B'].
       move: (H n ltac:(omega)) => [_ [h0 _]].
